TaplLean.lean
@@ -1,1 +1,1 @@
-import TaplLean.Basic
+import TaplLean.Chapter1
