TaplLean/Util.lean
@@ -1,8 +1,0 @@
--- Util.lean
-
-universe u
-
-class StepRel (α : Type u) where
-  step : α → α → Prop
-
-infixr:50 " -> " => StepRel.step
